%1\pr{23(45)678}9
\documentclass{book}
\usepackage[utf8]{inputenc}
\usepackage[english]{babel}
\usepackage[margin=0.3in]{geometry} % for margins

\usepackage{hyperref}
\hypersetup{
    colorlinks=true,
    linkcolor=blue,
    citecolor=green
    filecolor=cyan,
    urlcolor=magenta,
}

\urlstyle{same}

\usepackage{enumitem}
\setlist[enumerate]{align=left, %, label*=\arabic*.}
  leftmargin=3.0mm, %
  labelsep=3.0mm, %
  rightmargin=0.0mm, %
  listparindent=0.0mm, %
  labelwidth=0.0mm, %
  itemindent=0.0mm, %
}
\setlist[enumerate,1]{label=(\arabic*)}
\setlist[enumerate,2]{label=(\arabic{enumi}.\arabic*)}
\setlist[enumerate,3]{label=(\arabic{enumi}.\arabic{enumii}.\arabic*)}
\setlist[enumerate,4]{label=(\arabic{enumi}.\arabic{enumii}.\arabic{enumiii}.\arabic*)}
\setlist[enumerate,5]{label=(\arabic{enumi}.\arabic{enumii}.\arabic{enumiii}.\arabic{enumiv}.\arabic*)}
\setlist[enumerate,6]{label=(\arabic{enumi}.\arabic{enumii}.\arabic{enumiii}.\arabic{enumiv}.\arabic{enumv}.\arabic*)}
\setlist[enumerate,7]{label=(\arabic{enumi}.\arabic{enumii}.\arabic{enumiii}.\arabic{enumiv}.\arabic{enumv}.\arabic{enumvi}.\arabic*)}
\setlist[enumerate,8]{label=(\arabic{enumi}.\arabic{enumii}.\arabic{enumiii}.\arabic{enumiv}.\arabic{enumv}.\arabic{enumvi}.\arabic{enumvii}.\arabic*)}

\setlist{nolistsep,after=}
\setlistdepth{8}
\renewlist{itemize}{itemize}{8}
\renewlist{enumerate}{enumerate}{8}

\usepackage{amsmath}
\usepackage{bbold}
\usepackage{stix}
\usepackage{verbatim}

\usepackage{mleftright} % for left right
\mleftright
\delimitershortfall-1sp

\usepackage{xcolor}
\usepackage{framed}
\colorlet{shadecolor}{black!100} % \begin{shaded}\end{shaded}

\usepackage{silence}
\WarningFilter*{amsmath}{Foreign command}

%\usepackage{ocgx}

\newcommand{\df}[1]{\hypertarget{#1}{\textcolor{red}{#1}}}
\newcommand{\rf}[1]{\hyperlink{#1}{\textcolor{cyan}{#1}}}
%\newcommand{\df}[1]{#1}
%\newcommand{\rf}[1]{#1}
\newcommand{\abr}{:=}
\newcommand{\cont}{\phantom{.}. . .\phantom{.}}
\newcommand{\pipe}{$\phantom{(}\vrectangleblack\phantom{)}$}
\newcommand{\pr}[1]{\left(#1\right)}
\newcommand{\thmcontext}[1]{\centerline{\\************************ #1 ************************ \\}}


\usepackage{xifthen}% provides \isempty test
\newcommand{\ann}[2]{%
  \hfill %
  $\stackrel%
  {\hbox{\tiny{\ifthenelse{\isempty{#1}}%
    {\phantom{from}}%
    {from: $#1$}}}}%
  {\hbox{\tiny{\ifthenelse{\isempty{#2}}%
    {\phantom{wts}}%
    {wts: $#2$}}}}$%
\ }

\newcommand{\setbackgroundcolour}{\pagecolor[rgb]{0.2,0.2,0.2}}
\newcommand{\settextcolour}{\color[rgb]{0.8,0.8,0.8}}
\newcommand{\invertbackgroundtext}{\setbackgroundcolour\settextcolour}
\newcommand{\bbin}[1]{\mathbin{{\bar{#1}}}}
\newcommand{\st}{\mathbin{|}}
\newcommand{\utup}[1]{\{#1\}}
\newcommand{\notation}[2]{\fbox{{[Notation] \phantom{-} $#1 \abr #2$}}}
\newcommand{\floor}[1]{\left\lfloor #1 \right\rfloor}
\newcommand{\ceil}[1]{\left\lceil #1 \right\rceil}

%\usepackage[author={Max Schlepzig}]{pdfcomment}
%Here we\pdfcomment[icon=Insert]{insert: miss} a word!

\newenvironment{lit}{\item \vspace{.75mm} \hrule \vspace{.75mm}}

% "sumatra": "C:\\Users\\guzma\\Downloads\\PortableInstallations\\PortableGit\\usr\\bin\\echo.exe", "keep_focus_delay": 0
\begin{document}

\invertbackgroundtext
\setlength{\parindent}{0pt}

%\tableofcontents
%\chapter{Problem Set 1}
\section{Problem Set 2}
Suppose $(a_n)_{n \in \mathbb{N}}, (b_n)_{n \in \mathbb{N}}, (c_n)_{n \in \mathbb{N}} \in \mathfrak{c}(\mathbb{R})$ and $\lim \limits_{n \to \infty}{}(c_n) \neq 0$ and for any $n \in \mathbb{N}$, $c_n \neq 0$. \\ \\


1.) Prove $\lim \limits_{n \to \infty}{}(c) = c$: \\
Observe that $(c)_{n \in \mathbb{N}} = c (1)_{n \in \mathbb{N}}$. By Theorem 4, $\lim \limits_{n \to \infty}{}(c) = \lim \limits_{n \to \infty}{}(c * 1) = c \lim \limits_{n \to \infty}{}(1)$. Since $\lim \limits_{n \to \infty}{}(1) = 1$, $\lim \limits_{n \to \infty}{}(c) = c * 1 = c$.
$\hfill \blacksquare$ \\ \\


2.) Prove $\lim \limits_{n \to \infty}{}(|a_n|) = |\lim \limits_{n \to \infty}{}(a_n)|$: \\
Let $\epsilon > 0$. By the hypotheses, $(a_n)_{n \in \mathbb{N}}$ converges to some $a \in \mathbb{R}$. Furthermore, there exists an $N \in \mathbb{N}$ such that for any $n \geq N$, $|a_n - a| < \epsilon$. This with the reverse triangle inequality yields $||a_n| - |a|| \leq |a_n - a| < \epsilon$, for any $n \geq N$. By transitivity of the order relation on $\mathbb{R}$, $||a_n| - |a|| < \epsilon$, for any $n \geq N$. Therefore, $\lim \limits_{n \to \infty}{}(|a_n|) = |a| = |\lim \limits_{n \to \infty}{}(a_n)|$.
$\hfill \blacksquare$ \\ \\


3.) Prove $\lim \limits_{n \to \infty}{}(a_n - b_n) = \lim \limits_{n \to \infty}{}(a_n) - \lim \limits_{n \to \infty}{}(b_n)$: \\
Observe that $(a_n - b_n)_{n \in \mathbb{N}} = (a_n)_{n \in \mathbb{N}} + (-1) (b_n)_{n \in \mathbb{N}}$. By Theorem 4, $(-1) (b_n)_{n \in \mathbb{N}} \in \mathfrak{c}(\mathbb{R})$ and $\lim \limits_{n \to \infty}{}(a_n - b_n) = \lim \limits_{n \to \infty}{}(a_n + (-1) b_n) = \\
\lim \limits_{n \to \infty}{}(a_n) + (-1) \lim \limits_{n \to \infty}{}(b_n) = \lim \limits_{n \to \infty}{}(a_n) - \lim \limits_{n \to \infty}{}(b_n)$
$\hfill \blacksquare$ \\ \\


4.) Prove $\lim \limits_{n \to \infty}{}\left(\frac{a_n}{c_n}\right) = \frac{\lim \limits_{n \to \infty}{}(a_n)}{\lim \limits_{n \to \infty}{}(c_n)}$: \\
Observe that $\left(\frac{a_n}{c_n}\right)_{n \in \mathbb{N}} = (a_n)_{n \in \mathbb{N}} * \left(\frac{1}{c_n}\right)_{n \in \mathbb{N}}$. By the hypotheses, $(a_n)_{n \in \mathbb{N}}$ converges to some $a \in \mathbb{R}$ and $(c_n)_{n \in \mathbb{N}}$ converges to some $c \in \mathbb{R}$. We can apply Theorem 8 on $(c_n)_{n \in \mathbb{N}}$ since it satisfies the necessary assumptions. Thus, $\left(\frac{1}{c_n}\right)_{n \in \mathbb{N}} \in \mathfrak{c}(\mathbb{R})$ and $\lim \limits_{n \to \infty}{}\left(\frac{1}{c_n}\right) = \frac{1}{c}$. We can now apply Theorem 6 to get $\lim \limits_{n \to \infty}{}\left(\frac{a_n}{c_n}\right) = \lim \limits_{n \to \infty}{}\left(a_n * \frac{1}{c_n}\right) = \lim \limits_{n \to \infty}{}(a_n) * \lim \limits_{n \to \infty}{}\left(\frac{1}{c_n}\right) = a * \frac{1}{c} = \frac{\lim \limits_{n \to \infty}{}(a_n)}{\lim \limits_{n \to \infty}{}(c_n)}$.
$\hfill \blacksquare$ \\ \\


5.) Prove $\lim \limits_{n \to \infty}{}(a_n \lor b_n) = \lim \limits_{n \to \infty}{}(a_n) \lor \lim \limits_{n \to \infty}{}(b_n)$: \\
By the definition of the lattice operations,
\begin{align}
    (a_n \lor b_n)_{n \in \mathbb{N}} = \frac{1}{2} (a_n)_{n \in \mathbb{N}} + \frac{1}{2} (b_n)_{n \in \mathbb{N}} + \frac{1}{2} (|a_n - b_n|)_{n \in \mathbb{N}}
\end{align}

By the hypotheses, $(a_n)_{n \in \mathbb{N}}$ converges to some $a \in \mathbb{R}$ and $(b_n)_{n \in \mathbb{N}}$ converges to some $b \in \mathbb{R}$. Using Item 3, Item 2, and Theorem 4, we can say that the RHS of (1) must also be convergent, and we apply them on (1)
\begin{align}
    \lim \limits_{n \to \infty}{}(a_n \lor b_n) = \frac{1}{2} \lim \limits_{n \to \infty}{}(a_n) + \frac{1}{2} \lim \limits_{n \to \infty}{}(b_n) + \frac{1}{2} \lim \limits_{n \to \infty}{}(|a_n - b_n|) = \frac{1}{2}(a + b + |a - b|) = a \lor b = \lim \limits_{n \to \infty}{}(a_n) \lor \lim \limits_{n \to \infty}{}(b_n)
\end{align}
$\hfill \blacksquare$ \\ \\


6.) Prove $\lim \limits_{n \to \infty}{}(a_n \land b_n) = \lim \limits_{n \to \infty}{}(a_n) \land \lim \limits_{n \to \infty}{}(b_n)$: \\
By the definition of the lattice operations,
\begin{align}
    (a_n \land b_n)_{n \in \mathbb{N}} = \frac{1}{2} (a_n)_{n \in \mathbb{N}} + \frac{1}{2} (b_n)_{n \in \mathbb{N}} + \frac{-1}{2} (|a_n - b_n|)_{n \in \mathbb{N}}
\end{align}

By the hypotheses, $(a_n)_{n \in \mathbb{N}}$ converges to some $a \in \mathbb{R}$ and $(b_n)_{n \in \mathbb{N}}$ converges to some $b \in \mathbb{R}$. Using Item 3, Item 2, and Theorem 4, we can say that the RHS of (3) must also be convergent, and we apply them on (3)
\begin{align}
    \lim \limits_{n \to \infty}{}(a_n \land b_n) = \frac{1}{2} \lim \limits_{n \to \infty}{}(a_n) + \frac{1}{2} \lim \limits_{n \to \infty}{}(b_n) + \frac{-1}{2} \lim \limits_{n \to \infty}{}(|a_n - b_n|) = \frac{1}{2}(a + b - |a - b|) = a \land b = \lim \limits_{n \to \infty}{}(a_n) \land \lim \limits_{n \to \infty}{}(b_n)
\end{align}
$\hfill \blacksquare$ \\ \\


% \newpage

%%%%%%%%%%%%%%%%%%%%%%%%%%%%%%%%%%%%%%%%%%%%%%%%%%%%%%%%%%
%%%%%%%%%%%%%%%%%%%%%%%%%%%%%%%%%%%%%%%%%%%%%%%%%%%%%%%%%%
%%%%%%%%%%%%%%%%%%%%%%%%%%%%%%%%%%%%%%%%%%%%%%%%%%%%%%%%%%

%%%%%%%%%%%%%%%%%%%%%%%%%%%%%%%%%%%%%%%%%%%%%%%%%%%%%%%%%%
%%%%%%%%%%%%%%%%%%%%%%%%%%%%%%%%%%%%%%%%%%%%%%%%%%%%%%%%%%
%%%%%%%%%%%%%%%%%%%%%%%%%%%%%%%%%%%%%%%%%%%%%%%%%%%%%%%%%%


%%%%%%%%%%%%%%%%%%%%%%%%%%%%%%%%%%%%%%%%%%%%%%%%%%%%%%%%%%%%%%%%%%%%%%%%%%%%%%%%%%%%%%%%%%%%%%%%%%%%%%%%%%%%%%%%%%%%%%%%%%%%%%%%%%%%%%%%%%%%%%%%%%%%%%%%%%%%%%%%%%%%%%%%%%%%%%%%%%%%%%%%%%%%%%%%%%%%%%%%%%%%%%%%%%%%%%%%%%%%%%%%%%%%%%%%%%%%%%%%%%%%%%%%%%%%%%%%%%%%%%%%%%%%%%%%%%%%%%%%%%%%%%%%%%%%%%%%%%%%%%%%%%%%%%%%%%%%%%%%%%%%%%%%%%%%%%%%%%%%%%%%%%%%
\end{document}

%############################################################################
% \left(\begin{array}{ll}
%   XXX \hfill \land \hfill \\
%   YYY \hfill \land \hfill \\
% \end{array}\right)
%############################################################################
