\documentclass{book}
\usepackage[utf8]{inputenc}
\usepackage[english]{babel}
\usepackage[margin=0.5in]{geometry} % for margins
 
\usepackage{hyperref}
\hypersetup{
    colorlinks=true,
    linkcolor=blue,
    citecolor=green
    filecolor=cyan,      
    urlcolor=magenta,
}

\urlstyle{same}

\usepackage{enumitem}
\setlist[enumerate]{align=left, %, label*=\arabic*.}
  leftmargin=3.0mm, %
  rightmargin=0.0mm, %
  listparindent=0.0mm, %
  labelwidth=0.0mm, %
  labelsep=0.0mm, %
  itemindent=0.0mm, %
}
\setlist[enumerate,1]{label=(\arabic*)\phantom{))}}
\setlist[enumerate,2]{label=(\arabic{enumi}.\arabic*)\phantom{))}}
\setlist[enumerate,3]{label=(\arabic{enumi}.\arabic{enumii}.\arabic*)\phantom{))}}
\setlist[enumerate,4]{label=(\arabic{enumi}.\arabic{enumii}.\arabic{enumiii}.\arabic*)\phantom{))}}
\setlist[enumerate,5]{label=(\arabic{enumi}.\arabic{enumii}.\arabic{enumiii}.\arabic{enumiv}.\arabic*)\phantom{))}}
\setlist[enumerate,6]{label=(\arabic{enumi}.\arabic{enumii}.\arabic{enumiii}.\arabic{enumiv}.\arabic{enumv}.\arabic*)\phantom{))}}
\setlist[enumerate,7]{label=(\arabic{enumi}.\arabic{enumii}.\arabic{enumiii}.\arabic{enumiv}.\arabic{enumv}.\arabic{enumvi}.\arabic*)\phantom{))}}
\setlist[enumerate,8]{label=(\arabic{enumi}.\arabic{enumii}.\arabic{enumiii}.\arabic{enumiv}.\arabic{enumv}.\arabic{enumvi}.\arabic{enumvii}.\arabic*)\phantom{))}}

\setlist{nolistsep,after=}
\setlistdepth{8}
\renewlist{itemize}{itemize}{8}
\renewlist{enumerate}{enumerate}{8}

\usepackage{amsmath}
\usepackage{bbold}
\usepackage{stix}

\usepackage{mleftright} % for left right
\mleftright
\delimitershortfall-1sp

\newcommand{\df}[1]{\hypertarget{#1}{\textcolor{red}{#1}}}
\newcommand{\wff}[1]{\hypertarget{#1}{\fbox{\textcolor{red}{#1}}\phantom{--}}}
\newcommand{\rf}[1]{\hyperlink{#1}{\textcolor{cyan}{#1}}}
%\newcommand{\df}[1]{#1}
%\newcommand{\wff}[1]{((#1))\phantom{--}}
%\newcommand{\rf}[1]{#1}
\newcommand{\abr}{:=}
\newcommand{\pipe}{$\phantom{(}\vrectangleblack\phantom{)}$}
\newcommand{\pr}[1]{\left(#1\right)}
\newcommand{\thmcontext}[1]{\centerline{\\ ************************ #1 ************************ \\}}

\usepackage{xifthen}% provides \isempty test
\newcommand{\ann}[2]{%
  \hfill %
  $\stackrel%
  {\hbox{\tiny{\ifthenelse{\isempty{#1}}%
    {\phantom{from}}%
    {from: #1}}}}%
  {\hbox{\tiny{\ifthenelse{\isempty{#2}}%
    {\phantom{wts}}%
    {wts: #2}}}}$%
\ }

\newcommand{\setbackgroundcolour}{\pagecolor[rgb]{0.2,0.2,0.2}}  
\newcommand{\settextcolour}{\color[rgb]{0.8,0.8,0.8}}    
\newcommand{\invertbackgroundtext}{\setbackgroundcolour\settextcolour}

%\usepackage[author={Max Schlepzig}]{pdfcomment}
%Here we\pdfcomment[icon=Insert]{insert: miss} a word!

\newenvironment{lit}{\item \vspace{.75mm} \hrule \vspace{.75mm}}

% "sumatra": "C:\\Users\\guzma\\Downloads\\PortableInstallations\\PortableGit\\usr\\bin\\echo.exe", "keep_focus_delay": 0
\begin{document}

\invertbackgroundtext 

\tableofcontents

\chapter{Philosopherers}
(1.5) \\
$\df{OrderTrichotomy}(<, S) \abr \forall_{x, y \in S}(x < y \veebar x = y \veebar y < x)$ \\
$\df{OrderTransitivity}(<, S) \abr \forall_{x, y, z \in S}\pr{(x < y \land y < z) \implies x < z}$ \\
$\df{Order}(<, S) \abr \rf{OrderTrichotomy}(<, S) \land \rf{OrderTransitivity}(<, S)$ \\

(1.7) \\
$\df{BoundedAbove}(E, S, <) \abr \rf{Order}(<, S) \land E \subset S \land \exists_{\beta \in S} \forall_{x \in E}(x \leq \beta)$ \\
$\df{BoundedBelow}(E, S, <) \abr \rf{Order}(<, S) \land E \subset S \land \exists_{\beta \in S} \forall_{x \in E}(\beta \leq x)$ \\
$\df{UpperBound}(\beta, E, S, <) \abr \rf{Order}(<, S) \land E \subset S \land \beta \in S \land \forall_{x \in E}(x \leq \beta)$ \\
$\df{LowerBound}(\beta, E, S, <) \abr \rf{Order}(<, S) \land E \subset S \land \beta \in S \land \forall_{x \in E}(\beta \leq x)$ \\

(1.8) \\
$\df{LUB}(\alpha, E, S, <) \abr \rf{UpperBound}(\alpha, E, S, <) \land \forall_{\gamma}\pr{\gamma < \alpha \implies \lnot \rf{UpperBound}(\gamma, E, S, <)}$ \\
$\df{GLB}(\alpha, E, S, <) \abr \rf{LowerBound}(\alpha, E, S, <) \land \forall_{\beta}\pr{\alpha < \beta \implies \lnot \rf{LowerBound}(\beta, E, S, <)}$ \\

(1.10) \\
$\df{LUBProperty}(S, <) \abr \forall_{E}\pr{\pr{\emptyset \neq E \subset S \land \rf{BoundedAbove}(E, S, <)} \implies \exists_{\alpha \in S}\pr{\rf{LUB}(\alpha, E, S, <)}}$ \\
$\df{GLBProperty}(S, <) \abr \forall_{E}\pr{\pr{\emptyset \neq E \subset S \land \rf{BoundedBelow}(E, S, <)} \implies \exists_{\alpha \in S}\pr{\rf{GLB}(\alpha, E, S, <)}}$ \\

(1.11) \\
\wff{LUBPropertyImpliesGLBProperty} $\rf{LUBProperty}(S, <) \implies \rf{GLBProperty}(S, <)$
\begin{enumerate}
  \lit $\rf{LUBProperty}(S, <) \implies \ldots$    \ann{}{2}
  \begin{enumerate}
    \lit $\pr{\emptyset \neq B \subset S \land \rf{BoundedBelow}(B, S, <)} \implies \ldots$    \ann{}{1.2}
    \begin{enumerate}
      \lit $\rf{Order}(<, S) \land \exists_{\delta' \in S}\pr{\rf{LowerBound}(\delta', B, S, <)}$    \ann{1.1}{}
      \lit $|B| = 1 \implies \ldots$    \ann{}{1.1.3}
      \begin{enumerate}
        \lit $\exists_{u'}(u' \in B)$ \pipe $u \abr choice(\{u' | u' \in B\})$ \pipe $B = \{u\}$ \pipe $\rf{GLB}(u, B, S, <)$    \ann{1.1.2}{}
        \lit $\exists_{\epsilon_0 \in S}\pr{\rf{GLB}(\epsilon_0, B, S, <)}$
      \end{enumerate}
      \lit $|B| = 1 \implies \exists_{\epsilon_0 \in S}\pr{\rf{GLB}(\epsilon_0, B, S, <)}$
      \lit $|B| \neq 1 \implies \ldots$    \ann{}{1.1.5}
      \begin{enumerate}
        \lit $\forall_{E}\pr{\pr{\emptyset \neq E \subset S \land \rf{BoundedAbove}(E, S, <)} \implies \exists_{\alpha \in S}\pr{\rf{LUB}(\alpha, E, S, <)}}$    \ann{1}{}
        \lit $L \abr \{s \in S | \rf{LowerBound}(s, B, S, <)\}$
        \lit $|B| > 1 \land \rf{OrderTrichotomy}(<, S)$ \pipe $\exists_{{b_1}' \in B} \exists_{{b_0}' \in B}({b_0}' < {b_1}')$    \ann{1.1.1}{1.1.4.7}
        \lit $b_1 \abr choice\pr{\{{b_1}' \in B | \exists_{{b_0}' \in B}({b_0}' < {b_1}')\}}$ \pipe $\lnot \rf{LowerBound}(b_1, B, S, <)$    \ann{1.1.4.2}{}
        \lit $b_1 \notin L$ \pipe $L \subset S$
        \lit $\delta \abr choice\pr{\{\delta' \in S | \rf{LowerBound}(\delta', B, S, <)\}}$ \pipe $\delta \in L$ \pipe $\emptyset \neq L$    \ann{1.1}{}
        \lit $\emptyset \neq L \subset S$
        \lit $\forall_{y \in L}\pr{\rf{LowerBound}(y, B, S, <)}$ \pipe $\forall_{y \in L} \forall_{x \in B}(y \leq x)$    \ann{1.1.4.2}{1.1.4.10}
        \lit $\forall_{x \in B}\pr{x \in S \land \forall_{y \in L}(y \leq x)}$ \pipe $\forall_{x \in B}\pr{\rf{UpperBound}(x, L, S, <)}$
        \lit $\exists_{x \in S}\pr{\rf{UpperBound}(x, L, S, <)}$ \pipe $\rf{BoundedAbove}(L, S, <)$
        \lit $\emptyset \neq L \subset S \land \rf{BoundedAbove}(L, S, <)$
        \lit $\exists_{\alpha' \in S}\pr{\rf{LUB}(\alpha', L, S, <)}$ \pipe $\alpha \abr choice\pr{\{\alpha' \in S | \pr{\rf{LUB}(\alpha', L, S, <)}\}}$    \ann{1.1.4.1}{1.1.4.21}
        \lit $\forall_{x}\pr{x \in B \implies \rf{UpperBound}(x, L, S, <)}$    \ann{1.1.4.9}{1.1.4.17}
        \lit $\forall_{x}\pr{\lnot \rf{UpperBound}(x, L, S, <) \implies x \notin B}$
        \lit $\gamma < \alpha \implies \ldots$    \ann{}{1.1.4.16}
        \begin{enumerate}
          \lit $\lnot \rf{UpperBound}(\gamma, L, S, <)$ \pipe $\gamma \notin B$    \ann{1.1.4.12, 1.1.4.14}{}
        \end{enumerate}
        \lit $\gamma < \alpha \implies \gamma \notin B$ \pipe $\gamma \in B \implies \gamma \geq \alpha$
        \lit $\forall_{\gamma \in B}(\alpha \leq \gamma)$ \pipe $\rf{LowerBound}(\alpha, B, S, <)$
        \lit $\alpha < \beta \implies \ldots$    \ann{}{1.1.4.19}
        \begin{enumerate}
          \lit $\forall_{y \in L}(y \leq \alpha < \beta)$ \pipe $\forall_{y \in L}(y \neq \beta)$   \ann{1.1.4.12}{}
          \lit $\beta \neq L$ \pipe $\lnot \rf{LowerBound}(\beta, B, S, <)$
        \end{enumerate}
        \lit $\alpha < \beta \implies \lnot \rf{LowerBound}(\beta, B, S, <)$ \pipe $\forall_{\beta \in S}\pr{\alpha < \beta \implies \lnot \rf{LowerBound}(\beta, B, S, <)}$
        \lit $\rf{LowerBound}(\alpha, B, S, <) \land \forall_{\beta \in S}\pr{\alpha < \beta \implies \lnot \rf{LowerBound}(\beta, B, S, <)}$    \ann{1.1.4.17, 1.1.4.19}{}
        \lit $\rf{GLB}(\alpha, B, S, <)$ \pipe $\exists_{\epsilon_1 \in S}\pr{\rf{GLB}(\epsilon_1, B, S, <)}$
      \end{enumerate}
      \lit $|B| \neq 1 \implies \exists_{\epsilon_1 \in S}\pr{\rf{GLB}(\epsilon_1, B, S, <)}$
    \lit $\pr{|B| = 1 \implies \exists_{\epsilon_0 \in S}\pr{\rf{GLB}(\epsilon_0, B, S, <)}} \land \pr{|B| \neq 1 \implies \exists_{\epsilon_1 \in S}\pr{\rf{GLB}(\epsilon_1, B, S, <)}}$    \ann{1.1.3, 1.1.5}{}
    \lit $(|B| = 1 \lor |B| \neq 1) \implies \exists_{\epsilon \in S}\pr{\rf{GLB}(\epsilon, B, S, <)}$ \pipe $\exists_{\epsilon \in S}\pr{\rf{GLB}(\epsilon, B, S, <)}$
    \end{enumerate}
    \lit $\pr{\emptyset \neq B \subset S \land \rf{BoundedBelow}(B, S, <)} \implies \exists_{\epsilon \in S}\pr{\rf{GLB}(\epsilon, B, S, <)}$
    \lit $\forall_{B}\pr{\pr{\emptyset \neq B \subset S \land \rf{BoundedBelow}(B, S, <)} \implies \exists_{\epsilon \in S}\pr{\rf{GLB}(\epsilon, B, S, <)}}$
    \lit $\rf{GLBProperty}(S, <)$
  \end{enumerate}
  \lit $\rf{LUBProperty}(S, <) \implies \rf{GLBProperty}(S, <)$ 
\end{enumerate} \vspace{.75mm} \hrule \vspace{.75mm} \ \\

(1.12) \\
$\df{Field}(F, +, *) \abr \exists_{\mathbb{0}, \mathbb{1} \in F} \forall_{x, y, z \in F}\left(\begin{array}{ll}
  x + y \in F \hfill \land \hfill x * y \in F \hfill \land \hfill \\
  x + y = y + x \hfill \land \hfill x * y = y * x \hfill \land \hfill \\
  (x + y) + z = x + (y + z) \hfill \land \hfill (x * y) * z = x * (y * z) \hfill \land \hfill \\
  \mathbb{1} \neq \mathbb{0} \hfill \land \hfill x * (y + z) = (x * y) + (x * z) \hfill \land \hfill \\
  \mathbb{0} + x = x \hfill \land \hfill \mathbb{1} * x = x \hfill \land \hfill \\
  \exists_{-x \in F} \pr{x + (-x) = \mathbb{0}} \hfill \land \hfill \pr{x \neq \mathbb{0} \implies \exists_{1/x \in F}\pr{x * (1/x) = \mathbb{1}}}
\end{array}\right)$ \\

\thmcontext{$\pr{\rf{Field}(F, +, *) \land x, y, z \in F} \implies \ldots$}
(1.14.a) \\
\wff{AdditiveCancellation} $(x + y = x + z) \implies y = z$
\begin{enumerate}
  \lit $y = \mathbb{0} + y = \pr{x + (-x)} + y = \pr{(-x) + x} + y = (-x) + (x + y) = \ldots$
  \lit $(-x) + (x + z) = \pr{(-x) + x} + z = \pr{x + (-x)} + z = \mathbb{0} + z = z$
\end{enumerate} \vspace{.75mm} \hrule \vspace{.75mm} \ \\

(1.14.b) \\
\wff{AdditiveIdentityUniqueness} $(x + y = x) \implies y = \mathbb{0}$ 
\begin{enumerate}
  \lit $x + y = x = \mathbb{0} + x = x + \mathbb{0}$
  \lit $y = 0$    \ann{\rf{AdditiveCancellation}}{}
\end{enumerate} \vspace{.75mm} \hrule \vspace{.75mm} \ \\

(1.14.c) \\
\wff{AdditiveInverseUniqueness} $(x + y = \mathbb{0}) \implies y = -x$
\begin{enumerate}
  \lit $x + y = \mathbb{0} = x + (-x)$
  \lit $y = -x$    \ann{\rf{AdditiveCancellation}}{}
\end{enumerate} \vspace{.75mm} \hrule \vspace{.75mm} \ \\

(1.14.d) \\
\wff{DoubleNegative} $x = -(-x)$
\begin{enumerate}
  \lit $\mathbb{0} = x + (-x) = (-x) + x$ \pipe $\mathbb{0} = (-x) + x$
  \lit $x = -(-x)$    \ann{\rf{AdditiveInverseUniqueness}}{}
\end{enumerate} \vspace{.75mm} \hrule \vspace{.75mm} \ \\

(1.15.a) \\
\wff{MultiplicativeCancellation} $(x \neq 0 \land x * y = x * z) \implies y = z$    \phantom{TODO}--- \\

(1.15.b) \\
\wff{MultiplicativeIdentityUniqueness} $(x \neq 0 \land x * y = x) \implies y = \mathbb{1}$    \phantom{TODO}--- \\

(1.15.c) \\
\wff{MultiplicativeInverseUniqueness} $(x \neq 0 \land x * y = \mathbb{1}) \implies y = 1/x$    \phantom{TODO}--- \\

(1.15.d) \\
\wff{DoubleReciprocal} $(x \neq 0) \implies x = 1/(1/x)$    \phantom{TODO}--- \\

(1.16.a) \\
\wff{Domination} $\mathbb{0} * x = \mathbb{0}$
\begin{enumerate}
  \lit $\mathbb{0} * x = (\mathbb{0} + \mathbb{0}) * x = \mathbb{0} * x + \mathbb{0} * x$ \pipe $\mathbb{0} * x =  \mathbb{0} * x + \mathbb{0} * x$
  \lit $\mathbb{0} * x = \mathbb{0}$    \ann{\rf{AdditiveIdentityUniqueness}}{}
\end{enumerate} \vspace{.75mm} \hrule \vspace{.75mm} \ \\

(1.16.b) \\
\wff{NonDomination} $(x \neq \mathbb{0} \land y \neq \mathbb{0}) \implies x * y \neq \mathbb{0}$
\begin{enumerate}
  \lit $(x \neq \mathbb{0} \land y \neq \mathbb{0}) \implies \ldots$
  \begin{enumerate}
    \lit $(x * y = 0) \implies \ldots$
    \begin{enumerate}
      \lit $\mathbb{1} = \mathbb{1} * \mathbb{1} = \pr{x * (1/x)} * \pr{y * (1/y)} = (x * y) * \pr{(1/x) * (1/y)} = \mathbb{0} * \pr{(1/x) * (1/y)} = \mathbb{0}$    \ann{1, 1.1, \rf{Domination}}{}
      \lit $\mathbb{1} = \mathbb{0} \land \mathbb{1} \neq \mathbb{0}$    $\smashtimes$
    \end{enumerate}
  \lit $(x * y = 0) \implies \bot$ \pipe $x * y \neq 0$
  \end{enumerate}
  \lit $(x \neq \mathbb{0} \land y \neq \mathbb{0}) \implies x * y \neq 0$
\end{enumerate} \vspace{.75mm} \hrule \vspace{.75mm} \ \\

(1.16.c) \\
\wff{NegationCommutativity} $(-x) * y = -(x * y) = x * (-y)$
\begin{enumerate}
  \lit $x * y + (-x) * y = (x + -x) * y = \mathbb{0} * y = \mathbb{0}$ \pipe $x * y + (-x) * y = \mathbb{0}$    \ann{\rf{Domination}}{2}
  \lit $(-x) * y = -(x * y)$    \ann{\rf{AdditiveInverseUniqueness}}{}
  \lit $x * y + x * (-y) = x * (y + -y) = x * \mathbb{0} = \mathbb{0}$ \pipe $x * y + x * (-y) = \mathbb{0}$    \ann{\rf{Domination}}{4}
  \lit $x * (-y) = -(x * y)$    \ann{\rf{AdditiveInverseUniqueness}}{}
  \lit $(-x) * y = -(x * y) = x * (-y)$    \ann{2, 4}{}
\end{enumerate} \vspace{.75mm} \hrule \vspace{.75mm} \ \\

(1.16.d) \\
\wff{NegativeMultiplication} $(-x) * (-y) = x * y$
\begin{enumerate}
  \lit $(-x) * (-y) = -\pr{x * (-y)} = -\pr{-(x * y)} = x * y$    \ann{\rf{NegationCommutativity}, \rf{DoubleNegative}}{}
\end{enumerate} \vspace{.75mm} \hrule \vspace{.75mm} \ \\

(1.17) \\
$\df{OrderedField}(F, +, *, <) \abr \left(\begin{array}{ll}
  \rf{Field}(F, +, *) \hfill \land \hfill \rf{Order}(<, F) \hfill \land \hfill \\
  \forall_{x, y, z \in F}(y < z \implies x + y < x + z) \hfill \land \hfill \\
  \forall_{x, y \in F}\pr{(x > \mathbb{0} \land y > \mathbb{0}) \implies x * y > \mathbb{0}}
\end{array}\right)$ \\

\thmcontext{$\pr{\rf{OrderedField}(F, +, *, <) \land x, y, z \in F} \implies \ldots$}
(1.18.a) \\
\wff{NegationFlipsOrder} $x > \mathbb{0} \iff -x < \mathbb{0}$
\begin{enumerate}
  \lit $x > \mathbb{0} \implies \ldots$
  \begin{enumerate}
    \lit $\mathbb{0} = (-x) + x > (-x) + \mathbb{0} = -x$ \pipe $\mathbb{0} > -x$ \pipe $-x < \mathbb{0}$
  \end{enumerate}
  \lit $x > \mathbb{0} \implies -x < \mathbb{0}$
  \lit $-x < \mathbb{0} \implies \ldots$
  \begin{enumerate}
    \lit $\mathbb{0} = x + (-x) < x + \mathbb{0} = x$ \pipe $\mathbb{0} < x$ \pipe $x > \mathbb{0}$
  \end{enumerate}
  \lit $-x < \mathbb{0} \implies x > \mathbb{0}$
  \lit $x > \mathbb{0} \implies -x < \mathbb{0} \land -x < \mathbb{0} \implies x > \mathbb{0}$ \pipe $x > \mathbb{0} \iff -x < \mathbb{0}$    \ann{2, 4}{}
\end{enumerate} \vspace{.75mm} \hrule \vspace{.75mm} \ \\

(1.18.a) \\
\wff{PositiveFactorPreservesOrder} $(x > \mathbb{0} \land y < z) \implies x * y < x * z$
\begin{enumerate}
  \lit $(x > \mathbb{0} \land y < z) \implies \ldots$
  \begin{enumerate}
    \lit $(-y) + z > (-y) + y = \mathbb{0}$ \pipe $z + (-y) = \mathbb{0}$
    \lit $x * (z + (-y)) > \mathbb{0}$ \pipe $x * z + x * (-y) > \mathbb{0}$
    \lit $x * z = \mathbb{0} + x * z = \pr{x * y + -(x * y)} + x * z = \pr{x * y + x * (-y)} + x * z = \ldots$    \ann{\rf{NegationCommutativity}}{}
    \lit $x * y + \pr{x * z + x * (-y)} > x * y + \mathbb{0} = x * y$    \ann{1.2}{}
    \lit $x * z > x * y$    \ann{1.3, 1.4}{}
  \end{enumerate}
    \lit $(x > \mathbb{0} \land y < z) \implies x * z > x * y$
\end{enumerate} \vspace{.75mm} \hrule \vspace{.75mm} \ \\













%%%%%%%%%%%%%%%%%%%%%%%%%%%%%%%%%%%%%%%%%%%%%%%%%%%%%%%%%%%%%%%%%%%%%%%%%%%%%%%%%%%%%%%%%%%%%%%%%%%%%%%%%%%%%%%%%%%%%%%%%%%%%%%%%%%%%%%%%%%%%%%%%%%%%%%%%%%%%%%%%%%%%%%%%%%%%%%%%%%%%%%%%%%%%%%%%%%%%%%%%%%%%%%%%%%%%%%%%%%%%
\chapter{First Chapter}

\begin{enumerate}
  \lit First
  \begin{enumerate}
    \lit Second
    \lit Third
  \end{enumerate}
  \lit Fourth
\end{enumerate}


This will be an empty chapter and I will put some text here

\begin{equation}
\label{eq:1}
\sum_{i=0}^{\infty} a_i x^i
\end{equation}

The equation \ref{eq:1} shows a sum that is divergent. This formula 
will later be used in the page \pageref{second}.

For further references \pipe see \href{http://www.sharelatex.com}{Something 
Linky} or go to the next url: \url{http://www.sharelatex.com} or open 
the next file \href{run:./file.txt}{File.txt}

It's also possible to link directly any word or 
\hypertarget{thesentence}{any sentence} in your document.
\df{supwithit}{Sup With It Theorem}

If you read this text, you will get no information.  Really?  
Is there no information?
\\ \\ \\ \\ \\ \\ \\ \\ \\ \\ \\ \\ \\ \\ \\ \\ \\ \\ \\ \\ \\ \\ \\ \\ \\ \\ \\ \\ \\ \\ \\ \\ \\ \\ \\ \\ \\ \\ \\ \\ \\ \\ \\ \\ 
For instance \hyperlink{thesentence}{this sentence}.
\rf{supwithit}
 
\end{document}